Start exercise 2

LambdaSub.v
@@ -1,4 +1,4 @@
-Require Import List String.
+Require Import List String Rewriting.
 Import ListNotations.
 Open Scope string_scope.
 
@@ -23,7 +23,7 @@ Inductive type :=
 | Top
 | Nat
 | Arr (τ τ' : type)
-| Rec (fds : list field)
+| Rec (fts : list field)
 with field :=
 | Fd (ℓ : label) (τ : type).
 
@@ -79,20 +79,18 @@ Notation "'λ' ( x : τ ) t" := (Abs x τ t)
  (format "'λ' ( x  :  τ )  t", at level 40, x at level 0, t at level 40) : terms_scope.
 Notation "{}" := (Rec []) : terms_scope.
 Notation "{ x ; .. ; y }" := (Rec (cons x .. (cons y []) ..))
- (format "{ x ;  .. ;  y }"): terms_scope.
+ (format "{ x ;  .. ;  y }") : terms_scope.
 Notation "t · ℓ" := (Acc t ℓ)
  (format "t · ℓ", at level 10) : terms_scope.
-Notation "ℓ  :  t" := (Fd ℓ t) : terms_scope.
+Notation "ℓ  =  t" := (Fd ℓ t) : terms_scope.
 
 Open Scope terms_scope.
 
-Example rectangle := {"dimensions" : {"width" : 20; "height" : 10}; "color" : 255}.
-Example foo := {"bar" : λ("f":nat→nat) λ("x":nat) rectangle}.
+Example rectangle := {"dimensions" = {"width" = 20; "height" = 10}; "color" = 255}.
+Example foo := {"bar" = λ("f":nat→nat) λ("x":nat) rectangle}.
 Example bar := <foo·"bar"> 42.
 
 End Terms.
-
-Import Terms.
 
 (** * Exercise 1 *)
 
@@ -101,8 +99,10 @@ Import Terms.
 (** Values are either variables, natural numbers, λ-abstractions, or records whose field "values"
     are themselves values. *)
 
-Definition get_label '(ℓ : _) := ℓ.
-Definition get_value '(_ : t) := t.
+Import Terms.
+
+Definition get_label '(ℓ = _) := ℓ.
+Definition get_value '(_ = t) := t.
 
 Inductive value : term -> Prop :=
 | value_var x : value (Var x)
@@ -119,6 +119,8 @@ Hint Constructors value : db.
     [Prop], it can be removed during extraction, and thus belongs strictly to the metatheoretical
     level. Therefore this approach would not scale to more complex developments, where the purpose
     is the extraction of a certified interpreter/compiler. *)
+
+Module Contexts.
 
 Inductive context :=
 | Nil
@@ -143,21 +145,26 @@ Notation "< t > C" := (RApp t C)
  (format "< t >  C", at level 30, t at level 40, only printing) : contexts_scope.
 Notation "< C > v { p }" := (LApp C v p)
  (format "< C >  v  { p }", at level 30, C at level 40, only printing) : contexts_scope.
-Notation "{ x }" := (Rec x []) : contexts_scope.
-Notation "{ x ; y ; .. ; z }" := (Rec x (cons y .. (cons z []) ..))
- (format "{ x ;  y ;  .. ;  z }") : contexts_scope.
+Notation "{| x |}" := (Rec x []) : contexts_scope.
+Notation "{| x ; y ; .. ; z |}" := (Rec x (cons y .. (cons z []) ..))
+ (format "{| x ;  y ;  .. ;  z |}") : contexts_scope.
 Notation "C · ℓ" := (Acc C ℓ)
  (format "C · ℓ", at level 10) : contexts_scope.
-Notation "ℓ  :  C" := (Fd ℓ C) : contexts_scope.
+Notation "ℓ  =  C" := (Fd ℓ C) : contexts_scope.
+Notation "t  =  u" := (eq t u) : core_scope. (* Redeclare eq notation *)
 
 Open Scope contexts_scope.
 
 Example rectangle :=
-  {"dimensions" : {"width" : []; ("height" : 10)%terms}; ("color" : 255)%terms}.
+  {|"dimensions" = {|"width" = []; ("height" = 10)%terms|}; ("color" = 255)%terms|}.
+
+End Contexts.
 
 (** ** Question 3 *)
 
 (** First, we need a function that tells us how to _fill_ a context. *)
+
+Import Contexts.
 
 Reserved Notation "C [ t ]" (at level 9, t at level 8).
 
@@ -166,7 +173,7 @@ Fixpoint fill_context C t :=
   | [] => t
   | RApp u C => <u> C[t]
   | LApp C u _ => <C[t]> u
-  | Rec (ℓ : C) fds => Terms.Rec (ℓ : C[t] :: fds)%terms
+  | Rec (ℓ = C) fds => Terms.Rec ((ℓ = C[t]) :: fds)%terms
   | C·ℓ => (C[t]·ℓ)%terms
   end
 where "C [ t ]" := (fill_context C t).
@@ -196,7 +203,7 @@ Fixpoint subst t u x :=
     if x =? y then t
     else if List.in_dec string_dec y (freevars u) then t
     else λ(y : τ) v[u/x]
-  | Terms.Rec fds => Terms.Rec (List.map (fun '(ℓ : v) => (ℓ : v[u/x])) fds)
+  | Terms.Rec fds => Terms.Rec (List.map (fun '(ℓ = v) => (ℓ = v[u/x])) fds)
   | v·ℓ => v[u/x]
   end
 where "t [ u / x ]" := (subst t u x) : terms_scope.
@@ -207,38 +214,162 @@ where "t [ u / x ]" := (subst t u x) : terms_scope.
     - [step] extends [reduce] to arbitrary evaluation contexts, and thus also implements _redex
       search_ *)
 
+Module Reductions.
+
 Reserved Infix "~>" (at level 50).
 
 Inductive reduce : term -> term -> Prop :=
-| RAppAbs x τ t v : value v ->
+
+| AppAbs x τ t v : value v ->
   <λ(x : τ) t> v ~> t[v/x]
-| RAccRec fds ℓ : value (Terms.Rec fds) ->
-  forall p : sig (fun w => List.find (fun '(ℓ' : _) => ℓ =? ℓ') fds = Some (ℓ : w)),
-  (Terms.Rec fds)·ℓ ~> proj1_sig p
+
+| AccRec fds ℓ v : value v ->
+  List.In (ℓ = v) fds ->
+  (Terms.Rec fds)·ℓ ~> v
+  
 where "t ~> u" := (reduce t u).
+
+Hint Constructors reduce : db.
 
 Reserved Infix "-->" (at level 50).
 
 Inductive step : term -> term -> Prop :=
-| RCtx C t u :
+
+| Ctx C t u :
   t ~> u ->
   C[t] --> C[u]
+
 where "t --> u" := (step t u).
 
-(** Some notations for the transitive closures of reductions that will be useful later. *)
+Hint Constructors step : db.
 
-Require Import Rewriting.
+(** Some notations for the transitive closures of reductions that will be useful later. *)
 
 Infix "~*>" := (multi reduce) (at level 50).
 Infix "-*->" := (multi step) (at level 50).
 
+Hint Constructors multi : db.
+
+End Reductions.
+
 (** ** Question 4 *)
+
+Import Reductions.
 
 Definition reducible t := exists u, t --> u.
 
 Theorem step_redex :
-  forall t, reducible t -> exists C u, t = C[u].
+  forall t, reducible t -> exists C u, eq t C[u].
 Proof.
   destruct 1 as [? H]. destruct H. eauto.
 Qed.
 
+(** * Exercise 2 *)
+
+(** ** Question 1 *)
+
+Module Typing.
+
+Export Types.
+
+(** First we need typing contexts, with a well-formedness predicate [well_formed]. *)
+
+Inductive assumption :=
+| Assum (x : ident) (τ : type).
+
+Hint Constructors assumption : db.
+
+Definition context := list assumption.
+
+Declare Scope typing_scope.
+Delimit Scope typing_scope with typing.
+Bind Scope typing_scope with assumption context.
+
+Notation "x : τ" := (Assum x τ) : typing_scope.
+
+Open Scope typing_scope.
+
+Definition well_formed (Γ : context) :=
+  forall a a', List.In a Γ -> List.In a' Γ ->
+  let '(x : τ) := a in
+  let '(x' : τ') := a' in
+  x = x' -> τ = τ'.
+
+(** Typing rules are implemented with the inductive predicate [well_typed]. *)
+
+Reserved Notation "Γ ⊢ t : τ" (at level 10, t at level 0, τ at level 10).
+
+Inductive well_typed : context -> term -> type -> Prop :=
+
+| Var Γ x τ : well_formed Γ ->
+  List.In (x : τ) Γ ->
+  Γ ⊢ (Var x) : τ
+
+| Nat Γ n : well_formed Γ ->
+  Γ ⊢ (Terms.Nat n) : nat
+
+| App Γ t u τ τ' :
+  Γ ⊢ t : τ' → τ -> Γ ⊢ u : τ' ->
+  Γ ⊢ (<t> u) : τ
+
+| Abs Γ Γ' x t τ τ':
+  (Γ ++ [x : τ] ++ Γ')%list ⊢ t : τ' ->
+  (Γ ++ Γ')%list ⊢ (λ(x : τ) t) : τ → τ'
+
+(** (Record) rule *)
+
+| Rec Γ fds fts :
+  (forall ℓ t, List.In (ℓ = t)%terms fds -> exists τ, List.In (ℓ : τ)%types fts /\ Γ ⊢ t : τ) ->
+  Γ ⊢ (Terms.Rec fds) : Types.Rec fts
+
+(** (Field) rule *)
+
+| Acc Γ t ℓ τ fts :
+  Γ ⊢ t : Rec fts -> List.In (ℓ : τ)%types fts ->
+  Γ ⊢ (t·ℓ) : τ
+
+where "Γ ⊢ t : τ" := (well_typed Γ t τ) : typing_scope.
+
+Hint Constructors well_typed : db.
+
+Notation "⊢ t : τ" := ([] ⊢ t : τ) (at level 10, t at level 0, τ at level 10).
+
+End Typing.
+
+(** ** Question 2 *)
+
+Import Typing.
+
+Axiom succ : term.
+Axiom succ_typing : forall Γ, Γ ⊢ succ : nat → nat.
+
+Definition t22 τ := λ("f" : τ) <succ> ((<"f"> {"ℓ₁" = 31; "ℓ₂" = 73})·"ℓ₃").
+
+(** Canonical example of typing for [t22]. *)
+
+Example τ22 := ({"ℓ₁" : nat; "ℓ₂" : nat} → {"ℓ₃" : nat})%types.
+
+Example t22_typing : ⊢ (t22 τ22) : τ22 → nat.
+Proof.
+  unfold t22. eapply (Abs [] []). simpl.
+  econstructor.
+  * eapply succ_typing.
+  * econstructor.
+    - econstructor.
+      + econstructor.
+        ** unfold well_formed. firstorder.
+           destruct a, a'. congruence.
+        ** econstructor. econstructor.
+      + econstructor. firstorder.
+        ** exists nat. econstructor.
+           -- econstructor. congruence.
+           -- inversion H. econstructor.
+              unfold well_formed. firstorder.
+              destruct a, a'. congruence.
+        ** exists nat. econstructor.
+           -- right. econstructor. congruence.
+           -- inversion H. econstructor.
+              unfold well_formed. firstorder.
+              destruct a, a'. congruence.
+    - econstructor. congruence.
+Qed.
